Weidenbach_Book/Watched_Literals_Watch_List_Domain_Enumeration.thy
@@ -2,14 +2,13 @@ theory Watched_Literals_Watch_List_Domain_Enumeration
   imports Watched_Literals_Watch_List_Enumeration Watched_Literals.Watched_Literals_Watch_List_Domain
 begin
 
-context isasat_input_ops
-begin
+no_notation Ref.update ("_ := _" 62)
 
 fun propagate_unit_and_add_wl_D
   :: \<open>nat literal \<Rightarrow> nat twl_st_wl \<Rightarrow> nat twl_st_wl nres\<close>
 where
   \<open>propagate_unit_and_add_wl_D K (M, N, D, NE, UE, Q, W) = do {
-      ASSERT(-K \<in># \<L>\<^sub>a\<^sub>l\<^sub>l);
+      ASSERT(-K \<in># \<L>\<^sub>a\<^sub>l\<^sub>l (all_atms N (NE + UE)));
       RETURN (Propagated (-K) 0 # M, N, None, add_mset {#-K#} NE, UE, {#K#}, W)
     }\<close>
 
@@ -18,39 +17,70 @@ definition negate_mode_bj_unit_wl_D
 where
 \<open>negate_mode_bj_unit_wl_D = (\<lambda>S. do {
     (S, K) \<leftarrow> find_decomp_target_wl 1 S;
-    ASSERT(K \<in># \<L>\<^sub>a\<^sub>l\<^sub>l);
+    ASSERT(K \<in># \<L>\<^sub>a\<^sub>l\<^sub>l (all_atms_st S));
     propagate_unit_and_add_wl_D K S
   })\<close>
 
 abbreviation find_decomp_target_wl_D_ref
   :: \<open>nat twl_st_wl \<Rightarrow> ((nat twl_st_wl \<times> nat literal) \<times> (nat twl_st_wl \<times> nat literal)) set\<close> where
   \<open>find_decomp_target_wl_D_ref S \<equiv>
-     {((T, K), (T', K')). (T, T') \<in> Id \<and> (K, K') \<in> Id \<and> literals_are_\<L>\<^sub>i\<^sub>n T \<and>
+     {((T, K), (T', K')). (T, T') \<in> Id \<and> (K, K') \<in> Id \<and> literals_are_\<L>\<^sub>i\<^sub>n (all_atms_st S) T \<and>
         equality_except_trail_wl T S}\<close>
 
 lemma find_decomp_target_wl_D_find_decomp_target_wl:
   fixes S S' :: \<open>nat twl_st_wl\<close>
   assumes
-    SS': \<open>(S, S') \<in> {(S, S''). (S, S'') \<in> Id \<and> literals_are_\<L>\<^sub>i\<^sub>n S}\<close> and \<open>(a, a') \<in> Id\<close>
+    SS': \<open>(S, S') \<in> {(S, S''). (S, S'') \<in> Id \<and> literals_are_\<L>\<^sub>i\<^sub>n (all_atms_st S) S}\<close> and \<open>(a, a') \<in> Id\<close>
   shows
     \<open>find_decomp_target_wl a S \<le> \<Down>(find_decomp_target_wl_D_ref S) (find_decomp_target_wl a' S')\<close>
   using assms unfolding find_decomp_target_wl_def
-  by (cases S') (auto intro!: RES_refine simp: literals_are_\<L>\<^sub>i\<^sub>n_def blits_in_\<L>\<^sub>i\<^sub>n_def)
+  by (cases S', intro RES_refine, auto) (*TODO proof *)
+     (auto intro!:  simp: literals_are_\<L>\<^sub>i\<^sub>n_def blits_in_\<L>\<^sub>i\<^sub>n_def)
 
 lemma is_\<L>\<^sub>a\<^sub>l\<^sub>l_add_mset_already_in:
-  \<open>x \<in># N \<Longrightarrow> is_\<L>\<^sub>a\<^sub>l\<^sub>l (add_mset x N) \<longleftrightarrow>  is_\<L>\<^sub>a\<^sub>l\<^sub>l N\<close>
+  \<open>x \<in># N \<Longrightarrow> is_\<L>\<^sub>a\<^sub>l\<^sub>l \<A> (add_mset x N) \<longleftrightarrow>  is_\<L>\<^sub>a\<^sub>l\<^sub>l \<A> N\<close>
   using is_\<L>\<^sub>a\<^sub>l\<^sub>l_def by auto
 
+lemma in_all_lits_of_mm_in_\<L>\<^sub>a\<^sub>l\<^sub>l:
+  \<open>x2 \<in># all_lits_of_mm ({#mset (fst x). x \<in># ran_m am#} + (aoap)) \<Longrightarrow>
+       x2 \<in># \<L>\<^sub>a\<^sub>l\<^sub>l (atm_of `# all_lits am (aoap))\<close>
+  \<open>x2 \<in># all_lits_of_mm ({#mset (fst x). x \<in># ran_m am#} + (aoap)) \<Longrightarrow>
+       x2 \<in># \<L>\<^sub>a\<^sub>l\<^sub>l (all_atms am (aoap))\<close>
+  by (auto simp: \<L>\<^sub>a\<^sub>l\<^sub>l_def all_lits_def all_lits_of_mm_def all_atms_def)
+
+lemma all_lits_add_mset:
+  \<open>all_lits am (add_mset {#x2#} ap) = {#x2,-x2#} + all_lits am ap\<close>
+  by (auto simp: all_lits_def all_lits_of_mm_add_mset all_lits_of_m_add_mset)
+find_theorems literals_are_\<L>\<^sub>i\<^sub>n Propagated
+thm  all_lits_def
 lemma negate_mode_bj_unit_wl_D_negate_mode_bj_unit_wl:
   fixes S S' :: \<open>nat twl_st_wl\<close>
   assumes
-    SS': \<open>(S, S') \<in> {(S, S''). (S, S'') \<in> Id \<and> literals_are_\<L>\<^sub>i\<^sub>n S}\<close>
+    SS': \<open>(S, S') \<in> {(S, S''). (S, S'') \<in> Id \<and> literals_are_\<L>\<^sub>i\<^sub>n (all_atms_st S) S}\<close>
   shows
-    \<open>negate_mode_bj_unit_wl_D S \<le> \<Down> {(S, S''). (S, S'') \<in> Id \<and> literals_are_\<L>\<^sub>i\<^sub>n S}
+    \<open>negate_mode_bj_unit_wl_D S \<le> \<Down> {(S, S''). (S, S'') \<in> Id \<and> literals_are_\<L>\<^sub>i\<^sub>n (all_atms_st S) S}
        (negate_mode_bj_unit_wl S')\<close>
   unfolding negate_mode_bj_unit_wl_D_def negate_mode_bj_unit_wl_def
   using assms
   apply (refine_vcg find_decomp_target_wl_D_find_decomp_target_wl)
+  apply auto
+  apply (auto simp: mset_take_mset_drop_mset' uminus_\<A>\<^sub>i\<^sub>n_iff all_lits_of_mm_add_mset
+     all_lits_of_m_add_mset in_all_lits_of_mm_uminus_iff ASSERT_refine in_all_lits_of_mm_in_\<L>\<^sub>a\<^sub>l\<^sub>l
+      intro!: is_\<L>\<^sub>a\<^sub>l\<^sub>l_add_mset_already_in[THEN iffD2]  vcg_of_RETURN(1)[OF Pure.reflexive]
+      dest:(* in_all_lits_of_mm_uminusD *))
+      apply ( auto simp add: literals_are_\<L>\<^sub>i\<^sub>n_def blits_in_\<L>\<^sub>i\<^sub>n_def all_lits_add_mset
+        intro!: is_\<L>\<^sub>a\<^sub>l\<^sub>l_add_mset_already_in[THEN iffD2]
+        simp: 
+       simp del: is_\<L>\<^sub>a\<^sub>l\<^sub>l_all_lits_st_\<L>\<^sub>a\<^sub>l\<^sub>l literals_are_\<L>\<^sub>i\<^sub>n_set_mset_\<L>\<^sub>a\<^sub>l\<^sub>l)
+       prefer 3
+       supply [[unify_trace_failure]]
+       apply (rule is_\<L>\<^sub>a\<^sub>l\<^sub>l_add_mset_already_in[THEN iffD2])
+       thm is_\<L>\<^sub>a\<^sub>l\<^sub>l_add_mset_already_in[THEN iffD2]
+      prefer 2
+      term all_atms
+      apply (rule vcg_of_RETURN(2)[OF Pure.reflexive])
+      thm vcg_of_RETURN(2)[OF Pure.reflexive]
+      oops
   apply (auto simp: mset_take_mset_drop_mset' uminus_\<A>\<^sub>i\<^sub>n_iff all_lits_of_mm_add_mset
      all_lits_of_m_add_mset in_all_lits_of_mm_uminus_iff literals_are_\<L>\<^sub>i\<^sub>n_def blits_in_\<L>\<^sub>i\<^sub>n_def
       intro!: is_\<L>\<^sub>a\<^sub>l\<^sub>l_add_mset_already_in[THEN iffD2] dest:(* in_all_lits_of_mm_uminusD *))
@@ -58,7 +88,7 @@ lemma negate_mode_bj_unit_wl_D_negate_mode_bj_unit_wl:
 
 definition negate_mode_bj_nonunit_wl_D_inv:: \<open>nat twl_st_wl \<Rightarrow> bool\<close> where
 \<open>negate_mode_bj_nonunit_wl_D_inv S \<longleftrightarrow>
-   (negate_mode_bj_nonunit_wl_inv S \<and> literals_are_\<L>\<^sub>i\<^sub>n S)\<close>
+   (negate_mode_bj_nonunit_wl_inv S \<and> literals_are_\<L>\<^sub>i\<^sub>n (all_atms_st S) S)\<close>
 
 definition negate_mode_bj_nonunit_wl_D
   :: \<open>nat twl_st_wl \<Rightarrow> nat twl_st_wl nres\<close> where
@@ -71,45 +101,46 @@ definition negate_mode_bj_nonunit_wl_D
   })\<close>
 
 lemma is_\<L>\<^sub>a\<^sub>l\<^sub>l_add_all_lits_of_m:
-  \<open>is_\<L>\<^sub>a\<^sub>l\<^sub>l (all_lits_of_mm B) \<Longrightarrow> atms_of A \<subseteq> atms_of_mm B \<Longrightarrow> is_\<L>\<^sub>a\<^sub>l\<^sub>l (all_lits_of_m A + all_lits_of_mm B)\<close>
+  \<open>is_\<L>\<^sub>a\<^sub>l\<^sub>l \<A> (all_lits_of_mm B) \<Longrightarrow> atms_of A \<subseteq> atms_of_mm B \<Longrightarrow> is_\<L>\<^sub>a\<^sub>l\<^sub>l \<A> (all_lits_of_m A + all_lits_of_mm B)\<close>
   unfolding is_\<L>\<^sub>a\<^sub>l\<^sub>l_def
   by (auto simp: in_all_lits_of_m_ain_atms_of_iff in_all_lits_of_mm_ain_atms_of_iff)
 
 lemma literals_are_\<L>\<^sub>i\<^sub>n_propagate_nonunit_and_add_wl:
   assumes
-    lits: \<open>literals_are_\<L>\<^sub>i\<^sub>n T'\<close> and
+    lits: \<open>literals_are_\<L>\<^sub>i\<^sub>n \<A> T'\<close> and
     le: \<open>2 \<le> count_decided (get_trail_wl S')\<close> and
     i': \<open>i' \<notin># dom_m (get_clauses_wl T')\<close> and
     atms: \<open>atms_of (DECO_clause (get_trail_wl S'))
      \<subseteq> atms_of_ms ((\<lambda>x. mset (fst x)) ` set_mset (ran_m (get_clauses_wl T'))) \<union>
-        atms_of_mm (get_unit_init_clss_wl T')\<close>
-  shows \<open>literals_are_\<L>\<^sub>i\<^sub>n
+        atms_of_mm (get_unit_init_clss_wl T')\<close> and
+    b: \<open>b \<longleftrightarrow> length (DECO_clause_l (get_trail_wl S')) = 2\<close>
+  shows \<open>literals_are_\<L>\<^sub>i\<^sub>n \<A>
           (M',
            fmupd i' (DECO_clause_l (get_trail_wl S'), b) (get_clauses_wl T'), None,
            get_unit_init_clss_wl T', get_unit_learned_clss_wl T', Q, (get_watched_wl T')
-           (DECO_clause_l (get_trail_wl S') ! 0 :=
+           ((DECO_clause_l (get_trail_wl S') ! 0) :=
               get_watched_wl T' (DECO_clause_l (get_trail_wl S') ! 0) @
-              [(i', DECO_clause_l (get_trail_wl S') ! Suc 0)],
-          DECO_clause_l (get_trail_wl S') ! Suc 0 :=
+              [(i', DECO_clause_l (get_trail_wl S') ! Suc 0, b)],
+          (DECO_clause_l (get_trail_wl S') ! Suc 0) :=
             get_watched_wl T' (DECO_clause_l (get_trail_wl S') ! Suc 0) @
-            [(i', DECO_clause_l (get_trail_wl S') ! 0)]))\<close>
-  (is \<open>literals_are_\<L>\<^sub>i\<^sub>n ?S\<close>) and
+            [(i', DECO_clause_l (get_trail_wl S') ! 0, b)]))\<close>
+  (is \<open>literals_are_\<L>\<^sub>i\<^sub>n \<A> ?S\<close>) and
   \<open>DECO_clause_l (get_trail_wl S') ! 0 = DECO_clause_l (get_trail_wl S') ! Suc 0 \<Longrightarrow>
-    literals_are_\<L>\<^sub>i\<^sub>n
+    literals_are_\<L>\<^sub>i\<^sub>n \<A>
      (M',
       fmupd i' (DECO_clause_l (get_trail_wl S'), True) (get_clauses_wl T'), None, get_unit_init_clss_wl T',
       get_unit_learned_clss_wl T', Q, (get_watched_wl T')
-      (DECO_clause_l (get_trail_wl S') ! 0 :=
+      ((DECO_clause_l (get_trail_wl S') ! 0) :=
          get_watched_wl T' (DECO_clause_l (get_trail_wl S') ! 0) @
-         [(i', DECO_clause_l (get_trail_wl S') ! 0), (i', DECO_clause_l (get_trail_wl S') ! 0)]))\<close>
-  (is \<open>?eq \<Longrightarrow> literals_are_\<L>\<^sub>i\<^sub>n ?S'\<close>)
+         [(i', DECO_clause_l (get_trail_wl S') ! 0, b), (i', DECO_clause_l (get_trail_wl S') ! 0, b)]))\<close>
+  (is \<open>?eq \<Longrightarrow> literals_are_\<L>\<^sub>i\<^sub>n \<A> ?S'\<close>)
 proof -
-  have lall: \<open>is_\<L>\<^sub>a\<^sub>l\<^sub>l (all_lits_of_mm ((\<lambda>C. mset (fst C)) `# ran_m (get_clauses_wl T')
+  have lall: \<open>is_\<L>\<^sub>a\<^sub>l\<^sub>l \<A> (all_lits_of_mm ((\<lambda>C. mset (fst C)) `# ran_m (get_clauses_wl T')
         + get_unit_clauses_wl T'))\<close> and
     blits: \<open>blits_in_\<L>\<^sub>i\<^sub>n T'\<close>
-    using lits unfolding literals_are_\<L>\<^sub>i\<^sub>n_def
+    using lits unfolding literals_are_\<L>\<^sub>i\<^sub>n_def all_lits_def
     by fast+
-  have \<open>is_\<L>\<^sub>a\<^sub>l\<^sub>l (all_lits_of_mm ((\<lambda>C. mset (fst C)) `# ran_m (get_clauses_wl ?S)
+  have \<open>is_\<L>\<^sub>a\<^sub>l\<^sub>l \<A> (all_lits_of_mm ((\<lambda>C. mset (fst C)) `# ran_m (get_clauses_wl ?S)
         + get_unit_clauses_wl ?S))\<close>
     using i' atms
     by (auto simp: ran_m_mapsto_upd_notin all_lits_of_mm_add_mset
@@ -123,11 +154,11 @@ proof -
         in_all_lits_of_mm_ain_atms_of_iff all_conj_distrib
         watched_by_alt_def get_unit_clauses_wl_alt_def
         simp del: DECO_clause_l_DECO_clause)
-  ultimately show \<open>literals_are_\<L>\<^sub>i\<^sub>n ?S\<close>
-    unfolding literals_are_\<L>\<^sub>i\<^sub>n_def by blast
+  ultimately show \<open>literals_are_\<L>\<^sub>i\<^sub>n \<A> ?S\<close>
+    unfolding literals_are_\<L>\<^sub>i\<^sub>n_def all_lits_def by blast
 
 
-  have \<open>is_\<L>\<^sub>a\<^sub>l\<^sub>l (all_lits_of_mm ((\<lambda>C. mset (fst C)) `# ran_m (get_clauses_wl ?S')
+  have \<open>is_\<L>\<^sub>a\<^sub>l\<^sub>l \<A> (all_lits_of_mm ((\<lambda>C. mset (fst C)) `# ran_m (get_clauses_wl ?S')
         + get_unit_clauses_wl ?S'))\<close>
     using i' atms
     by (auto simp: ran_m_mapsto_upd_notin all_lits_of_mm_add_mset
@@ -141,22 +172,22 @@ proof -
         in_all_lits_of_mm_ain_atms_of_iff all_conj_distrib
         watched_by_alt_def get_unit_clauses_wl_alt_def
         simp del: DECO_clause_l_DECO_clause)
-  ultimately show \<open>?eq \<Longrightarrow> literals_are_\<L>\<^sub>i\<^sub>n ?S'\<close>
-    unfolding literals_are_\<L>\<^sub>i\<^sub>n_def by blast
+  ultimately show \<open>?eq \<Longrightarrow> literals_are_\<L>\<^sub>i\<^sub>n \<A> ?S'\<close>
+    unfolding literals_are_\<L>\<^sub>i\<^sub>n_def all_lits_def by blast
 qed
 
 
 lemma propagate_nonunit_and_add_wl_propagate_nonunit_and_add_wl:
   assumes
     TK: \<open>(TK, TK') \<in> {((S, K), (S'', K'')). (K, K'') \<in> Id \<and> (S, S'') \<in> Id
-      \<and> literals_are_\<L>\<^sub>i\<^sub>n S}\<close> and
+      \<and> literals_are_\<L>\<^sub>i\<^sub>n \<A> S}\<close> and
     [simp]: \<open>TK = (T, K)\<close> and
     [simp]: \<open>TK' = (T', K')\<close> and
     \<open>(i, i') \<in> Id\<close> and
-    \<open>literals_are_\<L>\<^sub>i\<^sub>n T\<close> and
-    \<open>(S, S') \<in> {(S, S''). (S, S'') \<in> Id \<and> literals_are_\<L>\<^sub>i\<^sub>n S}\<close>
+    \<open>literals_are_\<L>\<^sub>i\<^sub>n \<A> T\<close> and
+    \<open>(S, S') \<in> {(S, S''). (S, S'') \<in> Id \<and> literals_are_\<L>\<^sub>i\<^sub>n \<A> S}\<close>
   shows \<open>propagate_nonunit_and_add_wl K (DECO_clause_l (get_trail_wl S)) i T
-         \<le> \<Down> {(S, S''). (S, S'') \<in> Id \<and> literals_are_\<L>\<^sub>i\<^sub>n S}
+         \<le> \<Down> {(S, S''). (S, S'') \<in> Id \<and> literals_are_\<L>\<^sub>i\<^sub>n \<A> S}
              (propagate_nonunit_and_add_wl K' (DECO_clause_l (get_trail_wl S')) i' T')\<close>
   using assms unfolding propagate_nonunit_and_add_wl_def
   by refine_vcg
@@ -169,14 +200,14 @@ lemma propagate_nonunit_and_add_wl_propagate_nonunit_and_add_wl:
 lemma negate_mode_bj_nonunit_wl_D_negate_mode_bj_nonunit_wl:
   fixes S S' :: \<open>nat twl_st_wl\<close>
   assumes
-    SS': \<open>(S, S') \<in> {(S, S''). (S, S'') \<in> Id \<and> literals_are_\<L>\<^sub>i\<^sub>n S}\<close>
+    SS': \<open>(S, S') \<in> {(S, S''). (S, S'') \<in> Id \<and> literals_are_\<L>\<^sub>i\<^sub>n \<A> S}\<close>
      (is \<open>_ \<in> ?input\<close>)
   shows
-    \<open>negate_mode_bj_nonunit_wl_D S \<le> \<Down>{(S, S''). (S, S'') \<in> Id \<and> literals_are_\<L>\<^sub>i\<^sub>n S}
+    \<open>negate_mode_bj_nonunit_wl_D S \<le> \<Down>{(S, S''). (S, S'') \<in> Id \<and> literals_are_\<L>\<^sub>i\<^sub>n \<A> S}
        (negate_mode_bj_nonunit_wl S')\<close>
 proof -
   have find_deomp: \<open>find_decomp_target_wl (count_decided (get_trail_wl S)) S
-    \<le> \<Down> {((S, K), (S'', K'')). (K, K'') \<in> Id \<and> (S, S'') \<in> Id \<and> literals_are_\<L>\<^sub>i\<^sub>n S}
+    \<le> \<Down> {((S, K), (S'', K'')). (K, K'') \<in> Id \<and> (S, S'') \<in> Id \<and> literals_are_\<L>\<^sub>i\<^sub>n \<A> S}
       (find_decomp_target_wl (count_decided (get_trail_wl S')) S')\<close>
       (is \<open>_ \<le> \<Down> ?find_d _\<close>)
     using SS' unfolding find_decomp_target_wl_def
@@ -208,12 +239,12 @@ definition negate_mode_restart_nonunit_wl_D_inv
  :: \<open>nat twl_st_wl \<Rightarrow> bool\<close>
 where
   \<open>negate_mode_restart_nonunit_wl_D_inv S \<longleftrightarrow>
-    (negate_mode_restart_nonunit_wl_inv S \<and>  literals_are_\<L>\<^sub>i\<^sub>n S)\<close>
+    (negate_mode_restart_nonunit_wl_inv S \<and>  literals_are_\<L>\<^sub>i\<^sub>n (all_atms_st S) S)\<close>
 
 definition restart_nonunit_and_add_wl_D_inv
   :: \<open>nat clause_l \<Rightarrow> nat \<Rightarrow> nat twl_st_wl \<Rightarrow> bool\<close>where
   \<open>restart_nonunit_and_add_wl_D_inv C i S \<longleftrightarrow>
-     restart_nonunit_and_add_wl_inv C i S \<and> literals_are_\<L>\<^sub>i\<^sub>n S\<close>
+     restart_nonunit_and_add_wl_inv C i S \<and> literals_are_\<L>\<^sub>i\<^sub>n (all_atms_st S) S\<close>
 
 fun restart_nonunit_and_add_wl_D
   :: \<open>nat clause_l \<Rightarrow> nat \<Rightarrow> nat twl_st_wl \<Rightarrow> nat twl_st_wl nres\<close>
@@ -240,7 +271,7 @@ where
 
 definition negate_mode_wl_D_inv :: \<open>nat twl_st_wl \<Rightarrow> bool\<close> where
   \<open>negate_mode_wl_D_inv S \<longleftrightarrow>
-  (negate_mode_wl_inv S \<and> literals_are_\<L>\<^sub>i\<^sub>n S)\<close>
+  (negate_mode_wl_inv S \<and> literals_are_\<L>\<^sub>i\<^sub>n (all_atms_st S) S)\<close>
 
 definition negate_mode_wl_D :: \<open>nat twl_st_wl \<Rightarrow> nat twl_st_wl nres\<close> where
   \<open>negate_mode_wl_D S = do {
@@ -256,7 +287,7 @@ definition negate_mode_wl_D :: \<open>nat twl_st_wl \<Rightarrow> nat twl_st_wl 
 
 lemma restart_nonunit_and_add_wl_D_restart_nonunit_and_add_wl:
   assumes
-    SS': \<open>(S, S') \<in> {(S, S''). (S, S'') \<in> Id \<and>  literals_are_\<L>\<^sub>i\<^sub>n S}\<close> and
+    SS': \<open>(S, S') \<in> {(S, S''). (S, S'') \<in> Id \<and>  literals_are_\<L>\<^sub>i\<^sub>n \<A> S}\<close> and
     inv: \<open>negate_mode_restart_nonunit_wl_inv S\<close> and
     \<open>(m, n) \<in> nat_rel\<close> and
     \<open>m \<in> {i. i < count_decided (get_trail_wl S)}\<close> and
@@ -266,7 +297,7 @@ lemma restart_nonunit_and_add_wl_D_restart_nonunit_and_add_wl:
     [simp]: \<open>TK' = (T', K')\<close> and
     ij: \<open>(i, i') \<in> {(i, j). i = j \<and> i \<notin># dom_m (get_clauses_wl S)}\<close>
   shows \<open>restart_nonunit_and_add_wl_D (DECO_clause_l (get_trail_wl S)) i T
-         \<le> \<Down>{(S, S''). (S, S'') \<in> Id \<and>  literals_are_\<L>\<^sub>i\<^sub>n S}
+         \<le> \<Down>{(S, S''). (S, S'') \<in> Id \<and>  literals_are_\<L>\<^sub>i\<^sub>n \<A> S}
             (restart_nonunit_and_add_wl (DECO_clause_l (get_trail_wl S')) i' T')\<close>
 proof -
   have [simp]: \<open>i = i'\<close> and j: \<open>i' \<notin># dom_m (get_clauses_wl S)\<close>
@@ -284,14 +315,14 @@ proof -
        restart_nonunit_and_add_wl_D_inv_def mset_take_mset_drop_mset'
         restart_nonunit_and_add_wl_inv_def
         equality_except_trail_wl_get_clauses_wl[symmetric]
-        intro!: is_\<L>\<^sub>a\<^sub>l\<^sub>l_add_all_lits_of_m )
+        intro!: is_\<L>\<^sub>a\<^sub>l\<^sub>l_add_all_lits_of_m)
     done
 qed
 
 lemma negate_mode_restart_nonunit_wl_D_negate_mode_restart_nonunit_wl:
   fixes S S' :: \<open>nat twl_st_wl\<close>
   assumes
-    SS': \<open>(S, S') \<in> {(S, S''). (S, S'') \<in> Id \<and> literals_are_\<L>\<^sub>i\<^sub>n S}\<close>
+    SS': \<open>(S, S') \<in> {(S, S''). (S, S'') \<in> Id \<and> literals_are_\<L>\<^sub>i\<^sub>n \<A> S}\<close>
   shows
     \<open>negate_mode_restart_nonunit_wl_D S \<le>
       \<Down> {(S, S''). (S, S'') \<in> Id \<and> literals_are_\<L>\<^sub>i\<^sub>n S}
@@ -328,11 +359,11 @@ qed
 lemma negate_mode_wl_D_negate_mode_wl:
   fixes S S' :: \<open>nat twl_st_wl\<close>
   assumes
-    SS': \<open>(S, S') \<in> {(S, S''). (S, S'') \<in> Id \<and> literals_are_\<L>\<^sub>i\<^sub>n S}\<close> and
+    SS': \<open>(S, S') \<in> {(S, S''). (S, S'') \<in> Id \<and> literals_are_\<L>\<^sub>i\<^sub>n \<A> S}\<close> and
     confl: \<open>get_conflict_wl S = None\<close>
   shows
     \<open>negate_mode_wl_D S \<le>
-      \<Down>  {(S, S''). (S, S'') \<in> Id \<and> literals_are_\<L>\<^sub>i\<^sub>n S}
+      \<Down>  {(S, S''). (S, S'') \<in> Id \<and> literals_are_\<L>\<^sub>i\<^sub>n \<A> S}
        (negate_mode_wl S')\<close>
 proof -
   show ?thesis
@@ -348,18 +379,13 @@ proof -
     done
 qed
 
-end \<comment> \<open>end of @{locale isasat_input_ops}\<close>
-
-context isasat_input_bounded_nempty
-begin
-
 context
   fixes P :: \<open>nat literal set \<Rightarrow> bool\<close>
 begin
 
 definition cdcl_twl_enum_inv_wl_D :: \<open>nat twl_st_wl \<Rightarrow> bool\<close> where
   \<open>cdcl_twl_enum_inv_wl_D S \<longleftrightarrow>
-    cdcl_twl_enum_inv_wl S \<and> literals_are_\<L>\<^sub>i\<^sub>n S\<close>
+    cdcl_twl_enum_inv_wl S \<and> literals_are_\<L>\<^sub>i\<^sub>n (all_atms_st S) S\<close>
 
 definition cdcl_twl_enum_wl_D :: \<open>nat twl_st_wl \<Rightarrow> bool nres\<close> where
   \<open>cdcl_twl_enum_wl_D S = do {
@@ -379,7 +405,7 @@ definition cdcl_twl_enum_wl_D :: \<open>nat twl_st_wl \<Rightarrow> bool nres\<c
 
 lemma cdcl_twl_enum_wl_D_cdcl_twl_enum_wl:
   assumes
-    SS': \<open>(S, S') \<in> {(S, S''). (S, S'') \<in> Id \<and> literals_are_\<L>\<^sub>i\<^sub>n S}\<close>
+    SS': \<open>(S, S') \<in> {(S, S''). (S, S'') \<in> Id \<and> literals_are_\<L>\<^sub>i\<^sub>n \<A> S}\<close>
   shows
     \<open>cdcl_twl_enum_wl_D S \<le> \<Down> bool_rel (cdcl_twl_enum_wl P S')\<close>
   unfolding cdcl_twl_enum_wl_D_def cdcl_twl_enum_wl_def
@@ -398,6 +424,5 @@ lemma cdcl_twl_enum_wl_D_cdcl_twl_enum_wl:
 
 end \<comment> \<open>end of context with \<^term>\<open>P\<close>\<close>
 
-end  \<comment> \<open>end of @{locale isasat_input_bounded_nempty}\<close>
 
 end
